\centerline{Steve Hsu\hfill homework 2}
\item{1.} a.

$$\eqalign{
101 &= 7(13) + 10\cr
13 &= 10 + 3\cr
10 &= 3(3) + 1\cr
3 &= 3(1)\cr
}$$
$\gcd (13, 101) = 1$

$1 = 10 - 3(3) = 10 - 3(13 - 10) = 10 - 3(13) + 3(10) =
4(10) - 3(13) = 4(101 - 7(13)) - 3(13) = 4(101) - 31(13)$

$x = -31, y = 4$
\medskip
\item{} b.

Since $31(13) \equiv 1 \pmod {101}$, $31 = 13^{-1} \pmod {101}$.
\bigskip
\item{2.}
$$\eqalign{
78192 &= 55931 + 22261\cr
55931 &= 2(22261) + 11409\cr
22261 &= 11409 + 10852\cr
11409 &= 10852 + 557\cr
10852 &= 19(557) + 269\cr
557 &= 2(269) + 19\cr
269 &= 14(19) + 3\cr
19 &= 6(3) + 1\cr
3 &= 3(1)\cr
}$$
$\gcd (78192, 55931) = 1$

$1 = 19 - 6(3) = 19 - 6(269 - 14(19)) = 85(19) - 6(269) =
85(557 - 2(269)) - 6(269) = 85(557) - 176(269) =
85(557) - 176(10852 - 19(557)) = 3429(557) - 176(10852) =
3429(11409 - 10852) - 176(10852) = 3429(11409) - 3605(10852) =
3429(11409) - 3605(22261 - 11409) = 7034(11409) - 3605(22261) =
7034(55931 - 2(22261)) - 3605(22261) = 7034(55931) - 17673(22261) =
7034(55931) - 17673(78192 - 55931) = 24707(55931) - 17673(78192)$

$x = -17673, y = 24707$
\bigskip
\item{3.} 
$$\eqalign{
4883 &= 4369 + 514\cr
4369 &= 8(514) + 257\cr
514 &= 2(257)\cr
}$$
$\gcd (4883, 4369) = 257$

$4883 = (19)(257), 4369 = (17)(257)$
\bigskip
\item{4.}
$$\eqalign{
10037 &= 13(743) + 378\cr
743 &= 378 + 365\cr
378 &= 365 + 13\cr
365 &= 28(13) + 1\cr
13 &= 13(1)\cr
}$$
$1 = 365 - 28(13) = 365 - 28(378 - 365) = 29(365) - 28(378) =
29(743 - 378) - 28(378) = 29(743) - 57(378) =
29(743) - 57(10037 - 13(743)) = 770(743) - 57(10037)$

$770 \equiv 743^{-1} \pmod {10037}$
\bigskip
\item{5.}
$$\eqalign{
7^2 &\equiv 49 \equiv 7 \pmod {21}\cr
7^4 &\equiv (7^2)^2 \equiv 7^2 \equiv 7 \pmod {21}\cr
7^8 &\equiv (7^4)^2 \equiv 7^2 \equiv 7 \pmod {21}\cr
7^{16} &\equiv (7^8)^2 \equiv 7^2 \equiv 7 \pmod {21}\cr
7^{32} &\equiv (7^{16})^2 \equiv 7^2 \equiv 7 \pmod {21}\cr
7^{64} &\equiv (7^{32})^2 \equiv 7^2 \equiv 7 \pmod {21}\cr
7^{128} &\equiv (7^{64})^2 \equiv 7^2 \equiv 7 \pmod {21}\cr
}$$
$7^{138} \equiv (7^{128})(7^8)(7^2) \equiv (7)(7)(7) \equiv (7)(7) \equiv 7 \pmod {21}$
\bigskip
\item{6.}
\proclaim Claim. If $p$ and $q$ are prime, then $\phi (pq) = (p - 1)(q - 1)$.

There is a total of $pq$ natural numbers less than or equal to $pq$.
Of these, $q$ integers ($p, 2p, \cdots, qp$) are multiples of $p$ and
$p$ integers ($q, 2q, \cdots, pq$) are multiples of $q$.
Only one ($pq$) is a multiple of both.
Since all integers except multiples of $p$ are relatively prime to $p$,
$\phi (pq) = pq - (p + q - 1) = (p - 1)(q - 1)$, as desired.
\bigskip
\item{7.}

Let $p = 4$ and $a = 3$.
Then $a^{p - 1} \equiv 3^{4 - 1} \equiv 3^3 \equiv 27 \equiv 3 \pmod 4$.
\bye
